Kue/EvalTests.lean
@@ -67,4 +67,10 @@ theorem eval_non_cycle_reference_still_uses_target_value :
       == .struct [("x", .regular, .kind .int), ("y", .regular, .kind .int)] true) = true := by
   native_decide
 
+theorem eval_regular_field_reference_to_hidden :
+    (evalStructRefs
+      (resolveStructRefs (.struct [("_secret", .hidden, .prim (.string "x")), ("value", .regular, .ref "_secret")] true))
+      == .struct [("_secret", .hidden, .prim (.string "x")), ("value", .regular, .prim (.string "x"))] true) = true := by
+  native_decide
+
 end Kue
