testdata/cue/hidden_field_reference.cue
@@ -1,0 +1,4 @@
+x: {
+  _secret: "x"
+  value: _secret
+}
